## 递增递减运算符

* [基本语法](#基本语法)

### 基本语法

附例一：

```php
<?php

declare(strict_types = 1);

$foo = 6;

++$foo;
var_dump($foo); // int(7)

$foo++;
var_dump($foo); // int(8)

```

附例二：

```php
<?php

declare(strict_types = 1);

$foo = 6;
$bar = ++$foo;

var_dump($foo); // int(7)
var_dump($bar); // int(7)

```

附例三：

```php
<?php

declare(strict_types = 1);

$foo = 6;
$bar = $foo++;

var_dump($foo); // int(7)
var_dump($bar); // int(6)

```

附例四：

```php
<?php

declare(strict_types = 1);

$foo = 6;
$bar = $foo++ + ++$foo;

var_dump($foo); // int(8)
var_dump($bar); // int(14)

```

附例五：

```php
<?php

declare(strict_types = 1);

$foo = 6;
$bar = 2;
$baz = $foo++ + ++$bar;

var_dump($foo); // int(7)
var_dump($bar); // int(3)
var_dump($baz); // int(9)

```

附例六：

```php
<?php

declare(strict_types = 1);

$foo = 6;

--$foo;
var_dump($foo); // int(5)

$foo--;
var_dump($foo); // int(4)

```

附例七：

```php
<?php

declare(strict_types = 1);

$foo = 6;
$bar = --$foo;

var_dump($foo); // int(5)
var_dump($bar); // int(5)

```

附例八：

```php
<?php

declare(strict_types = 1);

$foo = 6;
$bar = $foo--;

var_dump($foo); // int(5)
var_dump($bar); // int(6)

```

附例九：

```php
<?php

declare(strict_types = 1);

$foo = 6;
$bar = $foo-- + --$foo;

var_dump($foo); // int(4)
var_dump($bar); // int(10)

```

附例十：

```php
<?php

declare(strict_types = 1);

$foo = 6;
$bar = 2;
$baz = $foo-- + --$bar;

var_dump($foo); // int(5)
var_dump($bar); // int(1)
var_dump($baz); // int(7)

```

